Rename and redefine a few things

Core/Logic.v
@@ -9,60 +9,68 @@ From Coq Require Import
   Logic.FunctionalExtensionality
   Logic.PropExtensionality.
 
-Definition Prec {E} VE F :=
+Definition Prec E VE F :=
   @InterState E F VE ->
   Trace (ThreadEvent F) ->
   Prop.
 
-Definition Relt {E} VE F :=
+Definition Relt E VE F :=
   @InterState E F VE -> Trace (ThreadEvent F) ->
   @InterState E F VE -> Trace (ThreadEvent F) ->
   Prop.
 
-Definition PrecCompose {E VE F} (P : @Prec E VE F) (R : Relt VE F) : Prec VE F :=
+Inductive RTC {E VE F} {R : Relt E VE F} : Relt E VE F :=
+| RTCRefl s ρ : RTC s ρ s ρ
+| RTCTrans s ρ t σ r τ :
+    R s ρ t σ ->
+    RTC t σ r τ ->
+    RTC s ρ r τ.
+Arguments RTC {E VE F} R.
+
+Definition PrecCompose {E VE F} (P : Prec E VE F) (R : Relt E VE F) : Prec E VE F :=
   fun t σ => exists s ρ, P s ρ /\ R s ρ t σ.
 
 Notation "R << G" := (PrecCompose R G) (left associativity, at level 38).
 
-Definition ReltCompose {E VE F} (R G : @Relt E VE F) : Relt VE F :=
+Definition ReltCompose {E VE F} (R G : Relt E VE F) : Relt E VE F :=
   fun s ρ r τ => exists t σ, R s ρ t σ /\ G t σ r τ.
 Notation "R >> G" := (ReltCompose R G) (right associativity, at level 39).
 
-Class HasImpl A :=
-  impl : A -> A -> Prop.
-Notation "P ==> Q" := (impl P Q) (right associativity, at level 41).
+Class HasSub A :=
+  sub : A -> A -> Prop.
+Notation "P ==> Q" := (sub P Q) (right associativity, at level 41).
 
-Global Instance implPrec E VE F : HasImpl (@Prec E VE F) :=
+Global Instance implPrec E VE F : HasSub (@Prec E VE F) :=
   fun P Q => forall s ρ, P s ρ -> Q s ρ.
 
-Global Instance implRelt E VE F : HasImpl (@Relt E VE F) :=
+Global Instance implRelt E VE F : HasSub (Relt E VE F) :=
   fun P Q => forall s ρ t σ, P s ρ t σ -> Q s ρ t σ.
 
 Class HasStable {E VE F} A :=
-  Stable : @Relt E VE F -> A -> Prop.
+  Stable : Relt E VE F -> A -> Prop.
 
-Global Instance stableRelt {E VE F} : HasStable (@Relt E VE F) :=
-  fun R Q => (R >> Q ==> Q) /\ (Q >> R ==> Q).
+Global Instance stableRelt {E VE F} : HasStable (Relt E VE F) :=
+  fun R Q => (RTC R >> Q ==> Q) /\ (Q >> RTC R ==> Q).
 
 Global Instance stablePrec {E VE F} : HasStable (@Prec E VE F) :=
-  fun R P => P << R ==> P.
+  fun R P => P << RTC R ==> P.
 
-Definition id {E VE F} : @Relt E VE F :=
+Definition id {E VE F} : Relt E VE F :=
   fun s ρ t σ => s = t /\ ρ = σ.
 
 Definition ptop {E VE F} : @Prec E VE F :=
   fun _ _ => True.
-Definition rtop {E VE F} : @Relt E VE F :=
+Definition rtop {E VE F} : Relt E VE F :=
   fun _ _ _ _ => True.
 
 Notation "ρ --> σ" := (exists t, AllRetEv t /\ LinRw (ρ ++ t) σ)
   (at level 20).
 
 Definition Commit {E VE F} VF i (impl : Impl E F)
-  (R G : @Relt E VE F)
+  (R G : Relt E VE F)
   (P : @Prec E VE F)
   (ev : @Event E)
-  (Q : @Relt E VE F) :=
+  (Q : Relt E VE F) :=
   forall s ρ t,
   LinToSpec ρ VF ->
   P s ρ ->
@@ -73,15 +81,15 @@ Definition Commit {E VE F} VF i (impl : Impl E F)
       ρ --> σ.
 
 Definition VerifyPrim {E VE F} VF i (impl : Impl E F)
-  (R G : @Relt E VE F)
+  (R G : Relt E VE F)
   (P : @Prec E VE F)
   (ev : @Event E)
-  (Q : @Relt E VE F) :=
+  (Q : Relt E VE F) :=
   Stable R P /\
   Stable R Q /\
   Commit VF i impl R G P ev Q.
 
-CoInductive VerifyProg {E VE F} VF i (impl : Impl E F) : @Relt E VE F -> @Relt E VE F -> forall (A: Type), @Prec E VE F -> Prog E A -> @Relt E VE F -> Prop :=
+CoInductive VerifyProg {E VE F} VF i (impl : Impl E F) : Relt E VE F -> Relt E VE F -> forall (A: Type), @Prec E VE F -> Prog E A -> Relt E VE F -> Prop :=
 | SafeReturn A v :
     VerifyProg VF i impl rtop id A ptop (Return v) id
 | SafeBind A B R G P QI QR S (m : E A) (k : A -> Prog E B) :
@@ -110,28 +118,16 @@ Definition TIdle {E VE F} (i : ThreadName) : @Prec E VE F :=
     fst s i = Idle /\
     true = even (length (@projAgent (@LEvent E F) i (map (fun e => (fst e, liftOEv (snd e))) ρ))).
 
-Definition TInvoke {E VE F} impl (i : ThreadName) Ret (m : F Ret) : @Relt E VE F :=
+Definition TInvoke {E VE F} impl (i : ThreadName) Ret (m : F Ret) : Relt E VE F :=
   fun s ρ t σ =>
     TIdle i s ρ /\
     σ = app ρ (cons (i, CallEv m) nil) /\
     InterStep (impl:=impl) i s (i, OCallEv m) t.
 
-Inductive ReltRTC {E VE F} {R : @Relt E VE F} : @Relt E VE F :=
-| RTCRefl s ρ : ReltRTC s ρ s ρ
-| RTCStep s ρ t σ : R s ρ t σ -> ReltRTC s ρ t σ
-| RTCTrans s ρ t σ r τ :
-    ReltRTC s ρ t σ ->
-    ReltRTC t σ r τ ->
-    ReltRTC s ρ r τ.
-Arguments ReltRTC {E VE F} R.
-
-Definition InvokeAny {E VE F} impl : @Relt E VE F :=
+Definition InvokeAny {E VE F} impl : Relt E VE F :=
   fun s ρ t σ => exists i Ret (m : F Ret), TInvoke impl i Ret m s ρ t σ.
 
-Definition InvokeMany {E VE F} impl :=
-  ReltRTC (@InvokeAny E VE F impl).
-
-Definition Returned {E VE F} (i : ThreadName) {Ret} (m : F Ret) : @Relt E VE F :=
+Definition Returned {E VE F} (i : ThreadName) {Ret} (m : F Ret) : Relt E VE F :=
   fun s ρ t σ =>
     s = t /\ ρ = σ /\
     exists (v : Ret), 
@@ -139,7 +135,7 @@ Definition Returned {E VE F} (i : ThreadName) {Ret} (m : F Ret) : @Relt E VE F :
       exists r,
         projAgent i σ = app r (cons (i, RetEv m v) nil).
 
-Definition TReturn {E VE F} (impl : Impl E F) (i : ThreadName) {Ret} (m : F Ret) : @Relt E VE F :=
+Definition TReturn {E VE F} (impl : Impl E F) (i : ThreadName) {Ret} (m : F Ret) : Relt E VE F :=
   fun s ρ t σ =>
     fst t i = Idle /\
     σ = ρ /\
@@ -147,20 +143,17 @@ Definition TReturn {E VE F} (impl : Impl E F) (i : ThreadName) {Ret} (m : F Ret)
       projAgent i σ = app r (cons (i, RetEv m v) nil) /\
       InterStep (impl:=impl) i s (i, ORetEv m v) t.
 
-Definition ReturnAny {E VE F} impl : @Relt E VE F :=
+Definition ReturnAny {E VE F} impl : Relt E VE F :=
   fun s ρ t σ => exists i Ret (m : F Ret), TReturn impl i m s ρ t σ.
-
-Definition ReturnMany {E VE F} impl :=
-  ReltRTC (@ReturnAny E VE F impl).
 
 Definition VerifyImpl
   {E F}
   (VE : Spec E)
   (VF : Spec F)
-  (R G : ThreadName -> @Relt E VE F)
+  (R G : ThreadName -> Relt E VE F)
   (P : ThreadName -> forall Ret, F Ret -> @Prec E VE F)
   (impl : Impl E F)
-  (Q : ThreadName -> forall Ret, F Ret -> @Relt E VE F) : Prop :=
+  (Q : ThreadName -> forall Ret, F Ret -> Relt E VE F) : Prop :=
   (forall i Ret (m : F Ret),
     VerifyProg VF i impl (R i) (G i)
       (P i Ret m << TInvoke impl i Ret m)
